theories/tree_borrows/read_reorder.v
@@ -1,0 +1,311 @@
+From iris.prelude Require Import prelude options.
+From stdpp Require Export gmap.
+From simuliris.tree_borrows Require Import disjoint defs lang_base lang notation bor_semantics tree tree_lemmas bor_lemmas steps_preserve tactics class_instances.
+From iris.prelude Require Import options.
+
+Fixpoint nsteps P (e : expr) σ e'' σ'' n : Prop := match n with
+  0 => e = e'' ∧ σ = σ''
+| S n => ∃ e' σ', prim_step P e σ e' σ' nil ∧ nsteps P e' σ' e'' σ'' n end.
+
+(* An extremely simple simulation relation: After n steps, all actions on one side are reproducible in the other *)
+Definition identical_states_after P e1 e2 σ n := 
+  ∀ e' σ', nsteps P e1 σ e' σ' n → nsteps P e2 σ e' σ' n.
+
+Definition source (x1 x2 : string) l1 tg1 sz1 l2 tg2 sz2 erest : expr :=
+  let: x1 := Copy (Place l1 tg1 sz1) in
+  let: x2 := Copy (Place l2 tg2 sz2) in
+  erest.
+
+Definition target (x1 x2 : string) l1 tg1 sz1 l2 tg2 sz2 erest : expr :=
+  let: x2 := Copy (Place l2 tg2 sz2) in
+  let: x1 := Copy (Place l1 tg1 sz1) in
+  erest.
+
+
+Ltac solve_sub_redexes_are_values :=
+  let K := fresh "K" in
+  let e' := fresh "e'" in
+  let Heq := fresh "Heq" in
+  let Hv := fresh "Hv" in
+  let IH := fresh "IH" in
+  let Ki := fresh "Ki" in
+  let Ki' := fresh "Ki'" in
+  intros K e' Heq Hv;
+  destruct K as [ | Ki K]; first (done);
+  exfalso; induction K as [ | Ki' K IH] in e', Ki, Hv, Heq |-*;
+  [destruct Ki; inversion Heq; subst; cbn in *;
+    try rewrite to_val_of_result in Hv; congruence
+  | eapply IH; first (by rewrite Heq);
+    rewrite language_to_val_eq; apply fill_item_no_result;
+      by rewrite -language_to_val_eq].
+
+Lemma list_destruct_snoc {A} (l : list A) :
+  l = nil ∨ ∃ xt xh, l = xh ++ [xt].
+Proof.
+  rewrite -(rev_involutive l).
+  destruct (rev l) as [|xt xh]; first by left.
+  right. simpl. by repeat eexists.
+Qed.
+
+Lemma prim_step_let_inv x e es e' P σ σ' tt :
+  prim_step P (let: x := e in es) σ e' σ' tt →
+  (∃ ev, language.to_val e = Some ev ∧ tt = nil ∧ σ' = σ ∧ e' = subst' x e es) ∨
+  ∃ ei', language.to_val e = None ∧ prim_step P e σ ei' σ' tt ∧ e' = (let: x := ei' in es)%E.
+Proof.
+  destruct (language.to_val e) as [ev|] eqn:Hev.
+  - intros H%prim_base_step.
+    2: solve_sub_redexes_are_values.
+    inversion H as [x1 x2 x3 x4 EE| x1 x2 x3 x4 x5 x6 x7 x8 x9 x10 EE]; simplify_eq.
+    2: by inversion EE.
+    inversion EE; simplify_eq. left. eexists. done.
+  - intros (K&e1'&e2'&He1&He2&H)%prim_step_inv.
+    destruct (list_destruct_snoc K) as [->|(xt & xh & ->)].
+    + simpl in *; simplify_eq.
+      inversion H as [x1 x2 x3 x4 EE| x1 x2 x3 x4 x5 x6 x7 x8 x9 x10 EE]; simplify_eq.
+      2: by inversion EE.
+      inversion EE; simplify_eq.
+      match goal with [HH : is_Some (to_result e) |- _ ] =>
+         rewrite -language_to_val_eq Hev in HH; by destruct HH end.
+    + subst e'. rewrite /= fill_app in He1.
+      destruct xt; simplify_eq.
+      replace (Let x e es) with (fill [LetEctx x es] e) in He1; last done.
+      simplify_eq. right. eexists.
+      rewrite /= fill_app /=.
+      split; first done.
+      split; last done.
+      eapply fill_prim_step. eapply base_prim_step. done.
+Qed.
+
+Lemma prim_step_copy_inv l tg sz P σ e' σ' tt :
+  prim_step P (Copy (Place l tg sz)) σ e' σ' tt →
+  (∃ v trs', e' = (#v)%E ∧ tt = nil ∧ read_mem l sz (shp σ) = Some v ∧ trees_contain tg (strs σ) l.1 ∧ apply_within_trees (memory_access AccessRead (scs σ) tg (l.2, sz)) l.1 (strs σ) = Some trs' ∧ sz ≠ 0 ∧ σ' = mkState (shp σ) trs' (scs σ) (snp σ) (snc σ))
+∨ (∃ v, e' = (#v)%E ∧ tt = nil ∧ read_mem l sz (shp σ) = Some v ∧ sz = 0 ∧ σ' = σ)
+∨ (e' = (#(replicate sz ☠%S))%E ∧ tt = nil ∧ is_Some (read_mem l sz (shp σ)) ∧ trees_contain tg (strs σ) l.1 ∧ apply_within_trees (memory_access AccessRead (scs σ) tg (l.2, sz)) l.1 (strs σ) = None ∧ σ' = σ).
+Proof.
+  intros H%prim_base_step.
+  2: solve_sub_redexes_are_values.
+  inversion H as [x1 x2 x3 x4 EE| x1 x2 x3 x4 x5 x6 x7 x8 x9 x10 ME IE]; simplify_eq.
+  1: by inversion EE.
+  inversion ME; simplify_eq.
+  - inversion IE; simplify_eq.
+    + left. do 2 eexists. done.
+    + right. left. eexists. do 4 (split; first done). by destruct σ.
+  - simpl in *.
+    inversion IE; simplify_eq. right. right.
+    do 5 (split; first done).
+    by destruct σ.
+Qed.
+
+Lemma subst_val_twice_exchange e x1 x2 v1 v2 :
+  x1 ≠ x2 →
+  subst x1 (#v1)%E (subst' x2 (#v2)%E e) = subst x2 (#v2)%E (subst' x1 (#v1)%E e).
+Proof.
+  intros Hne.
+  simpl.
+  refine ((fix IH (e:expr) {struct e} : subst x1 #v1 (subst x2 #v2 e) = subst x2 #v2 (subst x1 #v1 e) := _) e).
+  destruct e as [| | | | | | | | | | | | | | | | |? el| | ]; simpl; try (f_equal; by eapply IH).
+  - clear IH. rewrite !bool_decide_decide. do 2 destruct decide; simplify_eq; simpl.
+    + rewrite bool_decide_decide decide_True //.
+    + rewrite bool_decide_decide decide_True //.
+    + do 2 rewrite bool_decide_decide decide_False //.
+  - f_equal. 1: apply IH. f_equal. rewrite !bool_decide_decide. do 2 destruct decide; simplify_eq; simpl; done.
+  - f_equal. 1: eapply IH.
+    induction el as [|?? IHel]; first done.
+    + simpl. f_equal. 2: apply IHel. apply IH.
+Qed.
+
+Lemma read_reorder_onesided x1 x2 l1 tg1 sz1 l2 tg2 sz2 erest P σ :
+  state_wf σ →
+  x1 ≠ x2 →
+  identical_states_after P (source x1 x2 l1 tg1 sz1 l2 tg2 sz2 erest) (target x1 x2 l1 tg1 sz1 l2 tg2 sz2 erest) σ 4.
+Proof.
+  destruct l1 as [blk1 off1], l2 as [blk2 off2].
+  intros Hwf Hne.
+  intros e4 σ4 (e1' & σ1 & [(?&[=]&_)|(e1&_&[(v1&trs1&->&_&Hread1&Hcontain1&Happly1&Hne1&->)|[(v1&->&_&Hrd1&->&->)|(->&_&Hread1&Hcontains1&HapplyNone1&->)]]%prim_step_copy_inv&->)]%prim_step_let_inv & Hrst).
+  all: destruct Hrst as (e2 & σ2 & [(?&[= <-]&_&->&->)|(?&[=]&_)]%prim_step_let_inv & Hrst).
+  all: simpl in *|-.
+  all: destruct Hrst as (e3' & σ3 & [(?&[=]&_)|(e3&_&[(v3&trs3&->&_&Hread3&Hcontain3&Happly3&Hne2&->)|[(v3&->&_&Hrd3&->&->)|(->&_&Hread3&Hcontains3&HapplyNone3&->)]]%prim_step_copy_inv&->)]%prim_step_let_inv & Hrst).
+  all: simpl in *|-.
+  all: destruct Hrst as (e4' & σ4' & [(?&[= <-]&_&->&->)|(?&[=]&_)]%prim_step_let_inv & <- & <-).
+  all: rewrite /target. 
+  all: rewrite bool_decide_decide decide_True; last congruence.
+  all: do 2 change (subst' (BNamed ?a) ?b ?c) with (subst a b c). 
+  all: rewrite subst_val_twice_exchange //.
+  - (* read x1: succeed, read x2: succeed *)
+    odestruct CopyEvt_commutes as (y1&y2&y3&y4&HH1&HH2).
+    { econstructor. 1: eapply Hcontain1. 1: eapply Happly1. 1: done. }
+    { econstructor. 1: eapply Hcontain3. 1: eapply Happly3. 1: done. }
+    do 2 eexists. split.
+    { change (Let ?x2 ?a ?b) with (fill [LetEctx x2 b] a).
+      eapply fill_prim_step. eapply base_prim_step.
+      econstructor 2. 1: econstructor 3. 1: done.
+      eapply HH1. }
+    do 2 eexists. split.
+    { simpl. eapply base_prim_step.
+      econstructor 1. econstructor. 1: done. done. }
+    do 2 eexists. simpl. split.
+    { change (Let ?x2 ?a ?b) with (fill [LetEctx x2 b] a).
+      eapply fill_prim_step. eapply base_prim_step.
+      econstructor 2. 1: econstructor 3. 1: done. simpl. done. }
+    do 2 eexists. split.
+    { simpl. eapply base_prim_step.
+      econstructor 1. econstructor. 1: done. done. }
+    split; last done. rewrite bool_decide_decide decide_True //; congruence.
+  - (* read x1: succeed, read x2: zerosized *)
+    do 2 eexists. split.
+    { change (Let ?x2 ?a ?b) with (fill [LetEctx x2 b] a).
+      eapply fill_prim_step. eapply base_prim_step.
+      econstructor 2. 1: econstructor 3. 1: done.
+      econstructor; done. }
+    do 2 eexists. split.
+    { simpl. eapply base_prim_step.
+      econstructor 1. econstructor. 1: done. done. }
+    do 2 eexists. simpl. split.
+    { change (Let x1 ?a ?b) with (fill [LetEctx x1 b] a).
+      eapply fill_prim_step. eapply base_prim_step.
+      econstructor 2. 1: econstructor 3. 1: done. simpl.
+      econstructor; done. }
+    do 2 eexists. split.
+    { simpl. eapply base_prim_step.
+      econstructor 1. econstructor. 1: done. done. }
+    split; last done. rewrite bool_decide_decide decide_True //; congruence.
+  - (* read x1: succeed, read x2: fail *)
+    do 2 eexists. split.
+    { change (Let x2 ?a ?b) with (fill [LetEctx x2 b] a).
+      eapply fill_prim_step. eapply base_prim_step.
+      econstructor 2. 1: econstructor 4. 1: done.
+      econstructor; admit. }
+    (* this admit needs the theorem saying that if it fails after the other read has succeeded, it also succeeds earlier *)
+    do 2 eexists. split.
+    { simpl. eapply base_prim_step.
+      econstructor 1. econstructor. 1: done. done. }
+    do 2 eexists. simpl. split.
+    { change (Let x1 ?a ?b) with (fill [LetEctx x1 b] a).
+      eapply fill_prim_step. eapply base_prim_step.
+      econstructor 2. 1: econstructor 3. 1: done. simpl.
+      econstructor; done. }
+    do 2 eexists. split.
+    { simpl. eapply base_prim_step.
+      econstructor 1. econstructor. 1: done. done. }
+    split; last done. rewrite bool_decide_decide decide_True //; congruence.
+  - (* read x1: zerosized, read x2: succeed *)
+    do 2 eexists. split.
+    { change (Let x2 ?a ?b) with (fill [LetEctx x2 b] a).
+      eapply fill_prim_step. eapply base_prim_step.
+      econstructor 2. 1: simpl; econstructor 3. 1: done.
+      econstructor; done. }
+    do 2 eexists. split.
+    { simpl. eapply base_prim_step.
+      econstructor 1. econstructor. 1: done. done. }
+    do 2 eexists. simpl. split.
+    { change (Let x1 ?a ?b) with (fill [LetEctx x1 b] a).
+      eapply fill_prim_step. eapply base_prim_step.
+      econstructor 2. 1: econstructor 3. 1: done. simpl.
+      econstructor; done. }
+    do 2 eexists. split.
+    { simpl. eapply base_prim_step.
+      econstructor 1. econstructor. 1: done. done. }
+    split; last done. rewrite bool_decide_decide decide_True //; congruence.
+  - (* read x1: zerosized, read x2: zerosized *)
+    do 2 eexists. simplify_eq. split.
+    { change (Let x2 ?a ?b) with (fill [LetEctx x2 b] a).
+      eapply fill_prim_step. eapply base_prim_step.
+      econstructor 2. 1: econstructor 3. 1: done.
+      econstructor; done. }
+    do 2 eexists. split.
+    { simpl. eapply base_prim_step.
+      econstructor 1. econstructor. 1: done. done. }
+    do 2 eexists. simpl. split.
+    { change (Let x1 ?a ?b) with (fill [LetEctx x1 b] a).
+      eapply fill_prim_step. eapply base_prim_step.
+      econstructor 2. 1: econstructor 3. 1: done. simpl.
+      econstructor; done. }
+    do 2 eexists. split.
+    { simpl. eapply base_prim_step.
+      econstructor 1. econstructor. 1: done. done. }
+    split; last by destruct σ. rewrite bool_decide_decide decide_True //; congruence.
+  - (* read x1: zerosized, read x2: fail *)
+    do 2 eexists. split.
+    { change (Let x2 ?a ?b) with (fill [LetEctx x2 b] a).
+      eapply fill_prim_step. eapply base_prim_step.
+      econstructor 2. 1: econstructor 4. 1: done.
+      econstructor; done. }
+    do 2 eexists. split.
+    { simpl. eapply base_prim_step.
+      econstructor 1. econstructor. 1: done. done. }
+    do 2 eexists. simpl. split.
+    { change (Let x1 ?a ?b) with (fill [LetEctx x1 b] a).
+      eapply fill_prim_step. eapply base_prim_step.
+      econstructor 2. 1: econstructor 3. 1: done. simpl.
+      econstructor; done. }
+    do 2 eexists. split.
+    { simpl. eapply base_prim_step.
+      econstructor 1. econstructor. 1: done. done. }
+    split; last by destruct σ. rewrite bool_decide_decide decide_True //; congruence.
+  - (* read x1: fail, read x2: succeed *)
+    do 2 eexists. split.
+    { change (Let x2 ?a ?b) with (fill [LetEctx x2 b] a).
+      eapply fill_prim_step. eapply base_prim_step.
+      econstructor 2. 1: econstructor 3. 1: done.
+      econstructor; done. }
+    simpl.
+    do 2 eexists. split.
+    { simpl. eapply base_prim_step.
+      econstructor 1. econstructor. 1: done. done. }
+    do 2 eexists. simpl. split.
+    { change (Let x1 ?a ?b) with (fill [LetEctx x1 b] a).
+      eapply fill_prim_step. eapply base_prim_step.
+      econstructor 2. 1: econstructor 4. 1: done. simpl.
+      econstructor; admit. }
+    (* this admit needs the theorem saying that if it fails earlier, it fails also after the other read has succeeded *)
+    do 2 eexists. split.
+    { simpl. eapply base_prim_step.
+      econstructor 1. econstructor. 1: done. done. }
+    split; last by destruct σ. rewrite bool_decide_decide decide_True //; congruence.
+  - (* read x1: fail, read x2: zerosized *)
+    do 2 eexists. split.
+    { change (Let x2 ?a ?b) with (fill [LetEctx x2 b] a).
+      eapply fill_prim_step. eapply base_prim_step.
+      econstructor 2. 1: econstructor 3. 1: done.
+      econstructor; done. }
+    do 2 eexists. split.
+    { simpl. eapply base_prim_step.
+      econstructor 1. econstructor. 1: done. done. }
+    do 2 eexists. simpl. split.
+    { change (Let x1 ?a ?b) with (fill [LetEctx x1 b] a).
+      eapply fill_prim_step. eapply base_prim_step.
+      econstructor 2. 1: econstructor 4. 1: done. simpl.
+      econstructor; done. }
+    do 2 eexists. split.
+    { simpl. eapply base_prim_step.
+      econstructor 1. econstructor. 1: done. done. }
+    split; last by destruct σ. rewrite bool_decide_decide decide_True //; congruence.
+  - (* read x1: fail, read x2: fail *)
+    do 2 eexists. split.
+    { change (Let x2 ?a ?b) with (fill [LetEctx x2 b] a).
+      eapply fill_prim_step. eapply base_prim_step.
+      econstructor 2. 1: econstructor 4. 1: done.
+      econstructor; done. }
+    do 2 eexists. split.
+    { simpl. eapply base_prim_step.
+      econstructor 1. econstructor. 1: done. done. }
+    do 2 eexists. simpl. split.
+    { change (Let x1 ?a ?b) with (fill [LetEctx x1 b] a).
+      eapply fill_prim_step. eapply base_prim_step.
+      econstructor 2. 1: econstructor 4. 1: done. simpl.
+      econstructor; done. }
+    do 2 eexists. split.
+    { simpl. eapply base_prim_step.
+      econstructor 1. econstructor. 1: done. done. }
+    split; last by destruct σ. rewrite bool_decide_decide decide_True //; congruence.
+Admitted.
+
+Theorem read_reorder x1 x2 l1 tg1 sz1 l2 tg2 sz2 erest P σ :
+  state_wf σ →
+  x1 ≠ x2 →
+  identical_states_after P (source x1 x2 l1 tg1 sz1 l2 tg2 sz2 erest) (target x1 x2 l1 tg1 sz1 l2 tg2 sz2 erest) σ 4
+∧ identical_states_after P (target x1 x2 l1 tg1 sz1 l2 tg2 sz2 erest) (source x1 x2 l1 tg1 sz1 l2 tg2 sz2 erest) σ 4.
+Proof.
+  split.
+  all: eapply read_reorder_onesided; done.
+Qed.
